veric/expr_lemmas2.v
@@ -1,0 +1,357 @@
+Require Import msl.msl_standard.
+Require Import veric.base.
+Require Import msl.rmaps.
+Require Import msl.rmaps_lemmas.
+Require Import veric.compcert_rmaps.
+Require Import veric.Clight_lemmas.
+Require Import veric.expr.
+Require Export veric.environ_lemmas. 
+
+Import Cop.
+Import Cop2.
+
+Opaque tc_andp. (* This is needed otherwise certain Qeds take
+    forever in Coq 8.3.  *)
+
+Lemma eval_lvalue_ptr : forall rho e (Delta: tycontext) te ve ge,
+mkEnviron ge ve te = rho -> 
+typecheck_var_environ ve (var_types Delta) -> 
+typecheck_glob_environ ge (glob_types Delta) ->
+denote_tc_assert (typecheck_lvalue Delta e) rho ->
+eval_lvalue e rho = Vundef \/ exists base, exists ofs, eval_lvalue e rho  = Vptr base ofs.
+Proof. 
+intros.
+induction e; eauto.
+simpl. unfold eval_var. 
+remember (Map.get (ve_of rho) i). destruct o; try rewrite eqb_type_eq; intuition;
+try destruct p; try rewrite eqb_type_eq; simpl; try remember (type_eq t t0); try destruct s;
+simpl; try remember (negb (type_is_volatile t0));try destruct b0; auto;
+try solve[right; eauto].
+remember (ge_of rho i); try rewrite eqb_type_eq; simpl.
+destruct o; try rewrite eqb_type_eq; simpl; eauto.
+destruct p; try rewrite eqb_type_eq; simpl; eauto.
+if_tac; eauto.
+unfold typecheck_var_environ in *. simpl in H2.
+unfold get_var_type in *. 
+remember ((var_types Delta) ! i).
+destruct o. subst. simpl in H2.
+super_unfold_lift.
+try rewrite eqb_type_eq in *; simpl in *; intuition.
+symmetry in Heqo1.
+specialize (H0 i t1 Heqo1).
+destruct H0. congruence.
+remember ((glob_types Delta) ! i). destruct o; simpl in *; try congruence. 
+super_unfold_lift. right. 
+ unfold typecheck_glob_environ in H1.
+symmetry in Heqo2. 
+specialize (H1 _  _ Heqo2). destruct H1 as [b [? ?]].
+rewrite <- H in *.  simpl ge_of in Heqo0. rewrite H1 in *.
+inv Heqo0. eauto. inv H2. 
+
+
+
+simpl in *. intuition. super_unfold_lift. unfold force_ptr in *. 
+destruct (eval_expr e rho); eauto.
+
+simpl in *. super_unfold_lift.
+rewrite tc_andp_sound in *. simpl in *. 
+super_unfold_lift. rewrite tc_andp_sound in *. 
+simpl in *. super_unfold_lift.
+destruct H2 as [[? ?] ?]. 
+spec IHe; auto. destruct IHe. 
+unfold eval_field.
+destruct (eval_lvalue e rho); eauto;
+destruct (typeof e); try congruence; auto.
+destruct (field_offset i f); eauto.
+unfold eval_field.
+destruct (eval_lvalue e rho); eauto;
+destruct (typeof e); try congruence; auto;
+try destruct (field_offset i f); eauto.
+destruct (field_offset i f0); eauto.
+unfold offset_val; right; eauto.
+Qed. 
+ 
+Ltac unfold_tc_denote :=
+unfold denote_tc_nonzero in *;
+unfold isptr in *;
+unfold denote_tc_igt in *;
+unfold denote_tc_Zle in *;
+unfold denote_tc_Zge in *;
+unfold denote_tc_samebase in *;
+unfold denote_tc_nodivover in *;
+unfold denote_tc_initialized in *.
+
+
+Lemma typecheck_lvalue_Evar:
+  forall i t pt Delta rho, typecheck_environ Delta rho ->
+           denote_tc_assert (typecheck_lvalue Delta (Evar i t)) rho ->
+           is_pointer_type pt = true ->    
+           typecheck_val (eval_lvalue (Evar i t) rho) pt = true.
+Proof.
+intros.
+simpl in *. unfold eval_var.
+
+unfold typecheck_environ in H. 
+intuition. 
+destruct rho. 
+unfold typecheck_var_environ in *. unfold get_var_type in *. 
+
+remember ((var_types Delta) ! i).
+destruct o; try rewrite eqb_type_eq in *; simpl in *; intuition. 
+super_unfold_lift.
+remember (type_eq t t0). destruct s; intuition. 
+subst. remember (negb(type_is_volatile t0)).
+rewrite tc_andp_sound in *. simpl in *. super_unfold_lift.
+ destruct b; intuition. 
+clear H3. symmetry in Heqo.
+specialize (H i t0 Heqo).
+
+{destruct H. 
+rewrite H in *. rewrite <- Heqb. rewrite eqb_type_refl in *. destruct pt; auto.
+}
+{remember ((glob_types Delta) ! i). destruct o; try congruence.
+rewrite tc_andp_sound in *.  simpl in *. 
+simpl in *. super_unfold_lift. destruct H0. remember (eqb_type t (globtype g)).
+symmetry in Heqb. destruct b; simpl in *; try congruence. apply eqb_type_true in Heqb.
+subst. 
+unfold same_env in *. 
+symmetry in Heqo0.  specialize (H5 _ _ Heqo0). 
+destruct H5. simpl in *. unfold Map.get. rewrite H5. 
+unfold typecheck_glob_environ in *. destruct (H3 i g); auto. destruct H6. 
+rewrite H6. rewrite eqb_type_refl. auto.
+destruct pt; inv H1; reflexivity.
+destruct H5; congruence. inv H0.
+inv H0.
+} 
+Qed.
+
+Lemma typecheck_expr_sound_Efield:
+  forall Delta rho e i t
+  (H: typecheck_environ Delta rho)
+  (IHe: (denote_tc_assert (typecheck_expr Delta e) rho ->
+          typecheck_val (eval_expr e rho) (typeof e) = true) /\
+          (forall pt : type,
+          denote_tc_assert (typecheck_lvalue Delta e) rho ->
+          is_pointer_type pt = true -> 
+          typecheck_val (eval_lvalue e rho) pt = true))
+  (H0: denote_tc_assert (typecheck_expr Delta (Efield e i t)) rho),
+  typecheck_val (eval_expr (Efield e i t) rho) (typeof (Efield e i t)) = true.
+Proof.
+intros.
+simpl in *. super_unfold_lift.
+ unfold eval_field, offset_val, deref_noload in *.
+assert (MODE: access_mode t = By_reference) by (destruct (access_mode t); auto; hnf in H0; try contradiction).
+rewrite MODE in *.
+destruct IHe.
+destruct rho.
+repeat( rewrite tc_andp_sound in *; simpl in *; super_unfold_lift). 
+simpl in H0.
+super_unfold_lift. destruct H0 as [[?  ]?].
+revert H4; case_eq (type_is_volatile t); simpl; intros; try contradiction.
+clear H5.
+unfold typecheck_environ in H. 
+destruct H as [_ [Hve [Hge _]]]. 
+assert (PTR := eval_lvalue_ptr _ e Delta te ve ge (eq_refl _) Hve Hge H0).
+specialize (H2 t H0).
+spec H2. clear - MODE; destruct t; try destruct i; try destruct s; try destruct f; inv MODE; simpl; auto.
+destruct PTR.
+elimtype False; clear - H H2. rewrite H in H2; inv H2.
+destruct H as [b [ofs ?]]. 
+rewrite H in *.
+destruct (typeof e); intuition. 
+destruct (field_offset i f); intuition.
+Qed.
+
+Lemma typecheck_lvalue_sound_Efield:
+ forall Delta rho e i t pt
+ (H: typecheck_environ Delta rho)
+ (IHe: (denote_tc_assert (typecheck_expr Delta e) rho ->
+          typecheck_val (eval_expr e rho) (typeof e) = true) /\
+        (forall pt0 : type, denote_tc_assert (typecheck_lvalue Delta e) rho ->
+           is_pointer_type pt0 = true -> 
+         typecheck_val (eval_lvalue e rho) pt0 = true))
+  (H0: denote_tc_assert (typecheck_lvalue Delta (Efield e i t)) rho)
+  (H1: is_pointer_type pt = true),
+  typecheck_val (eval_lvalue (Efield e i t) rho) pt = true.
+Proof.
+intros.
+simpl in *.
+repeat( rewrite tc_andp_sound in *; simpl in *; super_unfold_lift).
+super_unfold_lift.
+ unfold eval_field,offset_val in *; intuition. 
+specialize  (H3 pt). intuition. remember rho.
+destruct e0.
+unfold typecheck_environ in *. intuition. clear H4 H9.
+rewrite Heqe0 in H0.
+assert (PTR := eval_lvalue_ptr _ e _ _ _ _ Heqe0 H H7).
+rewrite Heqe0 in *. clear Heqe0.
+intuition. 
+remember (eval_lvalue e rho). unfold isptr in *.
+destruct v; intuition; try congruence.
+remember (eval_lvalue e rho). destruct H8. destruct H4.
+destruct v; intuition; try congruence.
+inv H4.
+destruct (typeof e); intuition. 
+destruct (field_offset i f); intuition.
+Qed.
+
+Lemma typecheck_expr_sound_Evar:
+  forall Delta rho i t,
+  typecheck_environ Delta rho ->
+  denote_tc_assert (typecheck_expr Delta (Evar i t)) rho ->
+  typecheck_val (eval_expr (Evar i t) rho) (typeof (Evar i t)) = true.
+Proof.
+intros.
+assert (MODE: access_mode t = By_reference)
+ by (unfold typecheck_expr in H0; destruct (access_mode t); try (hnf in H0; contradiction); auto).
+simpl. super_unfold_lift. unfold deref_noload. rewrite MODE.
+
+ unfold typecheck_environ in H. intuition. 
+rename H4 into SM. 
+destruct rho. 
+unfold typecheck_var_environ, same_env in *.
+simpl in H0. rewrite MODE in H0.
+unfold get_var_type in *.
+
+remember ((var_types Delta) ! i).
+destruct o; try rewrite eqb_type_eq in *; simpl in *; intuition. 
+remember (type_eq t t0). destruct s; intuition. 
+subst. simpl in H0. 
+remember (negb(type_is_volatile t0)). destruct b; intuition. 
+clear H0. 
+symmetry in Heqo. 
+specialize (H i t0 Heqo).
+destruct H. unfold eval_var. simpl. 
+rewrite H in *. rewrite <- Heqb. rewrite eqb_type_refl in *.
+simpl. destruct t0; try destruct i0; try destruct s; try destruct f; inv MODE; auto.
+remember ((glob_types Delta) ! i). destruct o; try congruence. 
+simpl in *.
+rewrite tc_andp_sound in *. simpl in *. 
+unfold eval_var in *. 
+ super_unfold_lift. destruct H0. remember (eqb_type t (globtype g)).
+symmetry in Heqb. destruct b; simpl in *; try congruence. apply eqb_type_true in Heqb.
+subst. 
+symmetry in Heqo0.  specialize (SM _ _ Heqo0). 
+destruct SM. 
+unfold Map.get. rewrite H4. 
+unfold typecheck_glob_environ in *. 
+destruct (H2 i g); auto. destruct H5. 
+rewrite H5. rewrite eqb_type_refl. auto. destruct H4; congruence.
+inv H0. inv H0. 
+Qed.
+
+Lemma typecheck_unop_sound:
+ forall Delta rho u e t
+ (H: typecheck_environ Delta rho)
+ (IHe: (denote_tc_assert (typecheck_expr Delta e) rho ->
+          typecheck_val (eval_expr e rho) (typeof e) = true) /\
+          (forall pt : type,
+           denote_tc_assert (typecheck_lvalue Delta e) rho ->
+           is_pointer_type pt = true -> 
+           typecheck_val (eval_lvalue e rho) pt = true))
+  (H0: denote_tc_assert (typecheck_expr Delta (Eunop u e t)) rho),
+  typecheck_val (eval_expr (Eunop u e t) rho) (typeof (Eunop u e t)) = true.
+Proof.
+intros.
+simpl in H0. rewrite denote_tc_assert_andp in H0. destruct H0.
+destruct IHe as [? _].
+specialize (H2 H1).
+simpl eval_expr.
+unfold_lift.
+clear - H2 H0.
+revert H0; case_eq (isUnOpResultType u e t); intros; [ | inv H0].
+clear H0.
+simpl.
+forget (eval_expr e rho) as v.
+clear - H2 H.
+assert (TV: forall b i s a, typecheck_val (Val.of_bool b) (Tint i s a) = true)
+  by (destruct b; reflexivity).
+unfold isUnOpResultType in H.
+unfold eval_unop, sem_unary_operation, force_val1.
+unfold classify_bool in H.
+destruct u; try solve [inv H]; simpl.
+(* notbool case *)
+assert (is_int_type t = true) 
+  by (destruct (typeof e); try destruct i,s; inv H; auto).
+destruct t;  inv H0.
+unfold sem_notbool.
+destruct (typeof e), v; inv H2; try destruct i0,s0; simpl; inv H; try rewrite H1; auto.
+(* notint case *)
+unfold sem_notint.
+destruct (typeof e), v; inv H; inv H2; simpl; auto.
+destruct i,s; destruct t; inv H1; simpl; auto.
+(* neg case *)
+unfold sem_neg; simpl.
+destruct (typeof e); inv H.
+destruct v; inv H2.
+destruct i,s; inv H1; simpl; destruct t; try inv H0; auto.
+destruct v; inv H2.
+destruct f; inv H1; simpl; destruct t; try inv H0; auto.
+Qed.
+
+Lemma same_base_tc_val : forall v t1 t2,
+same_base_type t1 t2 = true ->
+typecheck_val v t1 = typecheck_val v t2.
+Proof.
+intros. destruct v; destruct t1; destruct t2; try solve [inv H]; auto.
+Qed.
+
+Lemma typecheck_temp_sound:
+  forall Delta rho i t,
+  typecheck_environ Delta rho ->
+  denote_tc_assert (typecheck_expr Delta (Etempvar i t)) rho ->
+  typecheck_val (eval_expr (Etempvar i t) rho) (typeof (Etempvar i t)) = true.
+Proof.
+intros.
+simpl in *. destruct rho. 
+destruct H as [H1 _].
+unfold typecheck_temp_environ in *.
+unfold eval_id, force_val in *. 
+
+simpl.
+destruct Delta as [[[? ?] ?] ?]. simpl in *.
+unfold temp_types in *. simpl in *.
+specialize (H1 i).
+destruct (type_is_volatile t); simpl in H0; unfold lift in H0; try contradiction.
+destruct (t0 ! i); try (contradiction H0).
+destruct p. destruct (H1 _ _ (eq_refl _)) as [v [? ?]]. clear H1.
+rewrite H.
+simpl in H0.
+remember (same_base_type t t4).
+destruct b0; [ | inv H0].
+
+simpl in H0.
+destruct b; inv H0;
+intuition;
+erewrite same_base_tc_val; eauto.
+simpl in H0. rewrite H in H0. inv H0.
+erewrite <- same_base_tc_val; eauto.
+Qed.
+
+Lemma typecheck_deref_sound:
+  forall Delta rho e t pt,
+   typecheck_environ Delta rho ->
+   (denote_tc_assert (typecheck_expr Delta e) rho ->
+    typecheck_val (eval_expr e rho) (typeof e) = true) /\
+    (forall pt0 : type,
+     denote_tc_assert (typecheck_lvalue Delta e) rho ->
+     is_pointer_type pt0 = true -> typecheck_val (eval_lvalue e rho) pt0 = true) ->
+     denote_tc_assert (typecheck_lvalue Delta (Ederef e t)) rho ->
+    is_pointer_type pt = true ->
+    typecheck_val (eval_lvalue (Ederef e t) rho) pt = true.
+Proof.
+intros until pt. intros H IHe H0 H1.
+simpl. unfold lift.
+simpl in H0.
+repeat rewrite denote_tc_assert_andp in H0.
+destruct H0 as [[[? ?] ?] ?].
+destruct IHe as[ ? _].
+specialize (H5 H0).
+revert H2; case_eq (is_pointer_type (typeof e)); intros; hnf in H2; try contradiction.
+clear H H6 H4.
+hnf in H3. unfold_lift in H3; hnf in H3.
+unfold_lift.
+destruct (eval_expr e rho); try contradiction.
+destruct pt; inv H1; reflexivity.
+Qed.
+
